feat: Wellfounded Recursion
- Wellfounded recursion
- Transfinite recursion
- Transitive closure of general relation
- Change definition of mem_trans_closure to a non-constructive universal-property definition (to avoid the cyclic dependency
    HOTG_Transfinite_Recursion -> HOTG_Less_Than -> HOTG_Mem_Transitive_Closure -> HOTG_Transfinite_Recursion)

HOTG/Mem_Transitive_Closure/HOTG_Mem_Transitive_Closure.thy
@@ -4,7 +4,7 @@ section \<open>Transitive Closure With Respect To Membership\<close>
 theory HOTG_Mem_Transitive_Closure
   imports
     HOTG_Foundation
-    HOTG_Transfinite_Recursion
+    HOTG_Mem_Transitive_Closed
 begin
 
 paragraph \<open>Summary\<close>
@@ -15,14 +15,94 @@ In particular, each such set is transitively closed.
 We follow the approach from \<^cite>\<open>ZFC_in_HOL_AFP\<close>,
 \<^url>\<open>https://foss.heptapod.net/isa-afp/afp-devel/-/blob/06458dfa40c7b4aaaeb855a37ae77993cb4c8c18/thys/ZFC_in_HOL/ZFC_Cardinals.thy#L410\<close>.\<close>
 
-definition "mem_trans_closure \<equiv> transrec (\<lambda>f X. X \<union> (\<Union>x \<in> X. f x))"
+definition "is_mem_trans_closure_of X T 
+  \<longleftrightarrow> (mem_trans_closed T \<and> X \<subseteq> T \<and> (\<forall>Y : mem_trans_closed. X \<subseteq> Y \<longrightarrow> T \<subseteq> Y))"
 
-lemma mem_trans_closure_eq_bin_union_idx_union:
+definition "mem_trans_closure X = (THE T. is_mem_trans_closure_of X T)"
+
+lemma is_mem_trans_closure_ofI:
+  assumes "mem_trans_closed T" "X \<subseteq> T" "\<And>Y. mem_trans_closed Y \<Longrightarrow> X \<subseteq> Y \<Longrightarrow> T \<subseteq> Y"
+  shows "is_mem_trans_closure_of X T"
+  using assms unfolding is_mem_trans_closure_of_def by blast
+
+lemma is_mem_trans_closure_ofE:
+  assumes "is_mem_trans_closure_of X T"
+  shows "mem_trans_closed T" "X \<subseteq> T" "\<And>Y. mem_trans_closed Y \<Longrightarrow> X \<subseteq> Y \<Longrightarrow> T \<subseteq> Y"
+  using assms unfolding is_mem_trans_closure_of_def by auto
+
+lemma eq_mem_trans_closure_if_is_mem_trans_closure_of:
+  assumes "is_mem_trans_closure_of X T"
+  shows "T = mem_trans_closure X"
+proof -
+  have "T = \<TT>" if "is_mem_trans_closure_of X \<TT>" for \<TT>
+    using assms that by (force elim: is_mem_trans_closure_ofE)
+  then have "\<exists>!T. is_mem_trans_closure_of X T" using assms by blast
+  from the1_equality[OF this] show ?thesis using assms mem_trans_closure_def by auto
+qed
+
+corollary is_mem_trans_closure_of_mem_trans_closure_if_is_mem_trans_closure_of:
+  assumes "is_mem_trans_closure_of X T"
+  shows "is_mem_trans_closure_of X (mem_trans_closure X)"
+  using assms eq_mem_trans_closure_if_is_mem_trans_closure_of by blast
+
+lemma has_mem_trans_closure_if_elements_have:
+  assumes trans_closure_elems: "\<And>x. x \<in> X \<Longrightarrow> is_mem_trans_closure_of x (mem_trans_closure x)"
+  defines "T \<equiv> X \<union> (\<Union>x \<in> X. mem_trans_closure x)"
+  shows "is_mem_trans_closure_of X T"
+proof (intro is_mem_trans_closure_ofI)
+  show "mem_trans_closed T"
+  proof (intro mem_trans_closedI)
+    fix z assume "z \<in> T"
+    then consider (mem) "z \<in> X" | (trans) x where "x \<in> X" "z \<in> mem_trans_closure x" using T_def by auto
+    then show "z \<subseteq> T"
+    proof cases
+      case mem
+      then have "z \<subseteq> mem_trans_closure z"
+        using trans_closure_elems is_mem_trans_closure_ofE mem_trans_closedD by auto
+      then show ?thesis using \<open>z \<in> X\<close> T_def by auto
+    next
+      case trans
+      then have "z \<subseteq> mem_trans_closure x" 
+        using trans_closure_elems is_mem_trans_closure_ofE mem_trans_closedD by auto
+      then show ?thesis using \<open>x \<in> X\<close> T_def by auto
+    qed
+  qed
+next
+  show "X \<subseteq> T" using T_def by auto
+next
+  fix Y assume hY: "mem_trans_closed Y" "X \<subseteq> Y"
+  show "T \<subseteq> Y"
+  proof
+    fix z assume "z \<in> T"
+    then consider (mem) "z \<in> X" | (trans) x where "x \<in> X" "z \<in> mem_trans_closure x" using T_def by auto
+    then show "z \<in> Y"
+    proof cases
+      case mem
+      then show ?thesis using \<open>X \<subseteq> Y\<close> by auto
+    next
+      case trans
+      then have "mem_trans_closure x \<subseteq> Y" 
+        using trans_closure_elems is_mem_trans_closure_ofE hY by blast
+      then show ?thesis using trans by auto
+    qed
+  qed
+qed
+
+theorem is_mem_trans_closure_of_mem_trans_closure: 
+  shows "is_mem_trans_closure_of X (mem_trans_closure X)"
+proof (induction X rule: mem_induction)
+  case (mem X)
+  then show ?case using has_mem_trans_closure_if_elements_have
+    using is_mem_trans_closure_of_mem_trans_closure_if_is_mem_trans_closure_of by blast
+qed
+
+corollary mem_trans_closure_eq_bin_union_idx_union:
   "mem_trans_closure X = X \<union> (\<Union>x \<in> X. mem_trans_closure x)"
-  by (simp add: mem_trans_closure_def transrec_eq[where ?X=X])
+  using has_mem_trans_closure_if_elements_have is_mem_trans_closure_of_mem_trans_closure
+  using eq_mem_trans_closure_if_is_mem_trans_closure_of[symmetric] by auto
 
 corollary subset_mem_trans_closure_self: "X \<subseteq> mem_trans_closure X"
-  by (auto simp: mem_trans_closure_eq_bin_union_idx_union[where ?X= X])
+  using is_mem_trans_closure_of_mem_trans_closure is_mem_trans_closure_ofE by auto
 
 corollary mem_mem_trans_closure_if_mem: "X \<in> Y \<Longrightarrow> X \<in> mem_trans_closure Y"
   using subset_mem_trans_closure_self by blast
@@ -48,22 +128,7 @@ lemma mem_trans_closure_eq_empty_iff_eq_empty [iff]: "mem_trans_closure X = {} \
   using subset_mem_trans_closure_self by auto
 
 lemma mem_trans_closed_mem_trans_closure: "mem_trans_closed (mem_trans_closure X)"
-proof (induction X)
-  case (mem X)
-  show ?case
-  proof (rule mem_trans_closedI')
-    fix x y assume "x \<in> mem_trans_closure X" "y \<in> x"
-    then show "y \<in> mem_trans_closure X"
-    proof (cases rule: mem_mem_trans_closureE)
-      case mem
-      have "y \<in> mem_trans_closure x" using \<open>y \<in> x\<close> subset_mem_trans_closure_self by blast
-      with mem show ?thesis by (subst mem_trans_closure_eq_bin_union_idx_union) blast
-    next
-      case mem_trans_closure
-      with \<open>y \<in> x\<close> mem.IH show ?thesis by (subst mem_trans_closure_eq_bin_union_idx_union) blast
-    qed
-  qed
-qed
+  using is_mem_trans_closure_of_mem_trans_closure is_mem_trans_closure_ofE by auto
 
 lemma not_mem_mem_trans_closure_self [iff]: "X \<notin> mem_trans_closure X"
 proof
@@ -77,11 +142,7 @@ qed
 
 lemma mem_trans_closure_le_if_le_if_mem_trans_closed:
   "mem_trans_closed X \<Longrightarrow> Y \<subseteq> X \<Longrightarrow> mem_trans_closure Y \<subseteq> X"
-proof (induction Y)
-  case (mem Y)
-  then show ?case
-    by (cases "Y = {}") (auto simp add: mem_trans_closure_eq_bin_union_idx_union[of Y])
-qed
+  using is_mem_trans_closure_of_mem_trans_closure is_mem_trans_closure_ofE(3) by blast
 
 lemma mem_trans_closure_subset_mem_trans_closure_if_subset:
   assumes "Y \<subseteq> X"
